Algsub/Parser.lean
@@ -1,0 +1,36 @@
+import Lean
+import Algsub.Basic
+
+open Lean Elab Meta
+
+declare_syntax_cat Term
+
+declare_syntax_cat Field
+syntax ident "=" Term : Field
+syntax Term : Field
+declare_syntax_cat NEFields
+syntax Field : NEFields
+syntax ident "=" Term "," NEFields : NEFields
+
+declare_syntax_cat Atom
+syntax "(" Term ")" : Atom
+syntax ident : Atom
+syntax num : Atom
+syntax "true" : Atom
+syntax "false" : Atom
+syntax "{}" : Atom
+syntax "{" NEFields "}" : Atom
+
+declare_syntax_cat PathTerm
+syntax PathTerm "." ident : PathTerm
+syntax Atom : PathTerm
+
+declare_syntax_cat AppTerm
+syntax PathTerm : AppTerm
+syntax AppTerm PathTerm : AppTerm
+
+syntax AppTerm : Term
+syntax "if" Term "then" Term "else" Term : Term
+syntax "let" ident "=" Term "in" Term : Term
+syntax "fun" ident "->" Term : Term
+syntax "fix" Term : Term
